cogent/llvm/checker/coq/Correctness.v
@@ -1,0 +1,240 @@
+From Coq Require Import List String ZArith.
+
+From ITree Require Import ITree ITreeFacts.
+From RecordUpdate Require Import RecordSet.
+From Vellvm Require Import LLVMAst LLVMEvents TopLevel Handlers InterpreterMCFG TopLevelRefinements
+  DynamicTypes CFG TypToDtyp InterpretationStack SymbolicInterpreter DenotationTheory ScopeTheory
+  DynamicValues ExpLemmas Coqlib NoFailure AListFacts.
+
+From Checker Require Import Denotation DenotationTheory Cogent Compiler Utils.Tactics Invariants
+  HelixLib.Correctness_Prelude HelixLib.BidBound.
+
+Import ListNotations.
+Import RecordSetNotations.
+Import AlistNotations.
+
+Definition vellvm_prog : Type := toplevel_entities typ (LLVMAst.block typ * list (LLVMAst.block typ)).
+Definition ocfg_res : Type := (block_id * block_id) + uvalue.
+
+Definition semantics_cogent (p : cogent_prog) : failT (itree E_mcfg) (memoryC * uval) := 
+  interp_cogent (denote_program p) "main" UUnit empty_memory.
+
+Import ExpTactics.
+Import ProofMode.
+
+Section Expressions.
+
+  (* From Helix *)
+  Definition branches (to : block_id) : Rel_cfg_T uval ocfg_res :=
+    fun _ '(m, (l, (g, res))) => exists from, res ≡ inl (from, to).
+
+  Definition compile_expr_post (i : im) (γ : ctx) (s1 s2 : IRState) (to : block_id)
+                               (l : local_env) : Rel_cfg_T uval ocfg_res :=
+    lift_Rel_cfg (state_invariant γ s2) ⩕
+    correct_result_T γ s1 s2 i ⩕
+    branches to ⩕
+    (fun _ '(_, (l', _)) => local_scope_modif s1 s2 l l').
+
+  Lemma compile_expr_correct :
+    forall (e : expr) (γ : ctx) (s1 s2 : IRState)
+           (v : im) (nextblock bid_in bid_from : block_id) (bks : ocfg typ)
+           (memC : memoryC) (g : global_env) (l : local_env) (memV : memoryV),
+      compile_expr e nextblock s1 ≡ inr (s2, (v, bid_in, bks)) ->
+      no_failure (interp_expr (E := E_cfg) (denote_expr γ e) memC) ->
+      bid_bound s1 nextblock ->
+      state_invariant γ s1 memC (memV, (l, g)) ->
+      eutt
+        (succ_cfg (compile_expr_post v γ s1 s2 nextblock l))
+        (interp_expr (denote_expr γ e) memC)
+        (interp_cfg (denote_ocfg (convert_typ [] bks) (bid_from,bid_in)) g l memV).
+  Proof.
+    induction e; intros * COMPILE NOFAIL NEXT PRE.
+    - (* compile_expr Unit *)
+      cbn* in *; simp.
+      cbn*.
+      rewrite denote_ocfg_unfold_not_in.
+      cvred.
+      apply eutt_Ret; split; [ | split; [ | split]]; cbn; eauto.
+      intros.
+      typ_to_dtyp_simplify.
+      unfold denote_exp; cbn.
+      go; reflexivity.
+      apply local_scope_modif_refl.
+      apply find_block_nil.
+    - (* compile_expr (Lit l) *)
+      cbn* in *; simp.
+      cbn*.
+      rewrite denote_ocfg_unfold_not_in.
+      cvred.
+      apply eutt_Ret; split; [ | split; [ | split]]; cbn; eauto.
+      intros.
+      destruct l;
+        simpl; typ_to_dtyp_simplify;
+        unfold denote_exp; cbn;
+        go; reflexivity.
+      apply local_scope_modif_refl.
+      apply find_block_nil.
+    - (* compile_expr (LVar i) *)
+      cbn* in *; simp.
+      rewrite denote_ocfg_unfold_not_in.
+      cvred.
+      unfold option_throw in *. simp.
+      cbn; cred.
+      apply eutt_Ret; split; [ | split; [ | split]]; cbn; eauto.
+      intros.
+      unfold id in *.
+      cbn* in *.
+      destruct PRE as [MEM WF].
+      unfold memory_invariant in MEM.
+      specialize (MEM _ _ _ Heqo0 Heqo).
+      unfold correct_result in MEM.
+      specialize (MEM l' H H0).
+      assumption.
+      apply local_scope_modif_refl.
+      apply failure_expr_throw in NOFAIL.
+      contradiction.
+      apply find_block_nil.
+    (* -
+      cbn* in COMPILE; simp.
+      unfold denote_expr, option_bind in *; cbn*; simp.
+      2 : apply failure_expr_throw in NOFAIL; contradiction.
+      rewrite interp_expr_Ret.
+      rewrite denote_code_nil.
+      vred.
+      apply eutt_Ret; split; [ | split]; cbn; eauto.
+      intros.
+      unfold id in *; cbn* in *.
+      destruct PRE as [MEM WF]; unfold memory_invariant in MEM.
+      specialize (MEM _ _ _ Heqo0 Heqo).
+      unfold equivalent_values in MEM.
+      specialize (MEM l' H H0).
+      assumption.
+    -
+      cbn* in *; simp.
+      rename s1 into pre_state, c0 into mid_state, c2 into post_state.
+      rename e0 into res_e1, e3 into res_e2, c1 into code_e1, c3 into code_e2.
+      rename Heqs into COMPILE_e1, Heqs0 into COMPILE_e2, e into op'.
+      vred.
+
+      specialize (IHe1 γ _ _ _ _ cogent_mem g l vellvm_mem COMPILE_e1).
+      forward IHe1; auto.
+      forward IHe1.
+      eapply no_failure_expr_bind_prefix; exact NOFAIL.
+      rewrite interp_expr_bind.
+      eapply eutt_clo_bind_returns ; [eassumption | clear IHe1].
+      introR; destruct_unit.
+      intros RET _; eapply no_failure_expr_bind_continuation in NOFAIL; [|eassumption]; clear RET.
+      cbn in PRE0.
+      destruct PRE0 as (PRE1 & [EXP1]).
+      cbn in *.
+
+      specialize (IHe2 γ _ _ _ _ memC g0 l0 memV COMPILE_e2).
+      forward IHe2; auto.
+      forward IHe2.
+      eapply no_failure_expr_bind_prefix; exact NOFAIL.
+      rewrite interp_expr_bind.
+      vred.
+      eapply eutt_clo_bind_returns ; [eassumption | clear IHe2].
+      introR; destruct_unit.
+      intros RET _; eapply no_failure_expr_bind_continuation in NOFAIL; [| eassumption];  clear RET.
+      destruct PRE0 as (PRE2 & [EXP2]).
+      cbn* in *.
+
+      specialize (EXP1 l1).
+      specialize (EXP2 l1).
+      forward EXP2.
+      red; reflexivity.
+      forward EXP2.
+      red; reflexivity.
+      forward EXP1.
+      {
+        admit.
+      }
+      forward EXP1.
+      {
+        admit.
+      }
+      admit.
+    -
+      cbn* in COMPILE; simp.
+      unfold denote_expr in *; cbn*.
+      rewrite interp_expr_Ret.
+      rewrite denote_code_nil.
+      vred.
+      apply eutt_Ret; split; [ | split]; cbn; eauto.
+      intros.
+      typ_to_dtyp_simplify.
+      unfold denote_exp; cbn.
+      go; reflexivity.
+    -
+      cbn* in COMPILE; simp.
+      unfold denote_expr in *; cbn*.
+      rewrite interp_expr_Ret.
+      rewrite denote_code_nil.
+      vred.
+      apply eutt_Ret; split; [ | split]; cbn; eauto.
+      intros.
+      destruct l;
+        simpl;
+        typ_to_dtyp_simplify;
+        unfold denote_exp; cbn;
+        go; reflexivity.
+    - 
+      cbn* in *; simp.
+      rename s1 into pre_state, c0 into mid_state, s2 into post_state.
+      rename Heqs into COMPILE_e1, Heqs0 into COMPILE_e2.
+      vred.
+
+      specialize (IHe1 γ _ _ _ _ cogent_mem g l vellvm_mem COMPILE_e1).
+      forward IHe1; auto.
+      forward IHe1.
+      eapply no_failure_expr_bind_prefix; exact NOFAIL.
+      rewrite interp_expr_bind.
+
+      (* might not need the following 3 *)
+      eapply eutt_clo_bind_returns ; [eassumption | clear IHe1].
+      introR; destruct_unit.
+      intros RET1 _; eapply no_failure_expr_bind_continuation in NOFAIL; [| eassumption]; clear RET1.
+      cbn in PRE0.
+      destruct PRE0 as (PRE1 & [EXP1]).
+      cbn in *.
+
+      specialize (IHe2 (vC :: γ) _ _ _ _ memC g0 l0 memV COMPILE_e2).
+      forward IHe2.
+      apply state_invariant_new_var; auto.
+      unfold equivalent_values.
+      intros.
+      specialize (EXP1 l'). *)
+      
+      
+      
+      
+      
+      
+      
+      
+      
+
+      
+
+      
+
+      
+      
+  Admitted.
+
+End Expressions.
+
+Section TopLevel.
+
+  (* placeholder *)
+  Definition TT {A B} (x: A) (y: B):= True.
+
+  Lemma compiler_correct :
+    forall (c : cogent_prog) (ll : vellvm_prog),
+      compile_cogent c ≡ inr ll ->
+      eutt TT (semantics_cogent c) (semantics_llvm ll).
+  Proof.
+  Abort.
+
+End TopLevel.
