cogent/llvm/checker/coq/DenotationTheory.v
@@ -1,0 +1,126 @@
+From ITree Require Import ITree Events.State Events.Exception Events.FailFacts Events.StateFacts
+  Interp.TranslateFacts Eq.Eq.
+
+From Vellvm Require Import Utils.NoFailure Utils.PropT.
+
+From Checker Require Import Denotation.
+
+Local Open Scope itree_scope.
+
+Section InterpTheory.
+
+  Lemma interp_mem_Ret :
+    forall T mem x,
+      @interp_mem T (Ret x) mem ≅ Ret (mem, x).
+  Proof.
+    intros T mem x.
+    unfold interp_mem.
+    apply interp_state_ret.
+  Qed.
+
+  Lemma interp_mem_bind :
+    forall T U mem (t : itree CogentL0 T) (k : T -> itree CogentL0 U),
+      interp_mem (ITree.bind t k) mem ≈ 
+        ITree.bind (interp_mem t mem) (fun '(mem', v) => interp_mem (k v) mem').
+  Proof.
+    intros; unfold interp_mem.
+    rewrite interp_state_bind.
+    apply eutt_eq_bind; intros []; reflexivity.
+  Qed.
+
+  Lemma interp_Mem_vis_eqit :
+    forall T R mem (e : CogentL0 T) (k : T -> itree CogentL0 R),
+      interp_mem (vis e k) mem ≅ ITree.bind ((case_ handle_mem pure_state) T e mem) (fun sx => Tau (interp_mem (k (snd sx)) (fst sx))).
+  Proof.
+    intros T R mem e k.
+    unfold interp_mem.
+    apply interp_state_vis.
+  Qed.
+
+  Lemma interp_expr_Ret :
+    forall E mem x,
+      @interp_expr E (Ret x) mem ≅ Ret (Some (mem, x)).
+  Proof.
+    intros.
+    unfold interp_expr.
+    rewrite interp_mem_Ret, interp_fail_Ret, translate_ret.
+    reflexivity.
+  Qed.
+
+  Lemma interp_expr_bind :
+    forall E mem (t : itree CogentL0 uval) (k : uval -> itree CogentL0 uval),
+      @interp_expr E (ITree.bind t k) mem ≈ 
+        ITree.bind (interp_expr t mem) (fun mx => 
+          match mx with 
+          (* | (a, b) => Ret None *)
+          | None => Ret None
+          | Some x => 
+              let '(mem',v) := x in 
+                interp_expr (k v) mem'
+          end).
+  Proof.
+    intros; unfold interp_expr.
+    rewrite interp_mem_bind, interp_fail_bind, translate_bind.
+    eapply eutt_eq_bind; intros [[]|]; cbn.
+    reflexivity.
+    rewrite translate_ret; reflexivity.
+  Qed.
+
+End InterpTheory.
+
+Section NoFailure.
+
+  Lemma no_failure_expr_Ret : forall E x m,
+    no_failure (interp_expr (E := E) (Ret x) m).
+  Proof.
+    intros.
+    rewrite interp_expr_Ret. apply eutt_Ret; intros abs; inv abs.
+  Qed.
+
+  Lemma failure_expr_throw : forall E s m,
+    ~ no_failure (interp_expr (E := E) (throw s) m).
+  Proof.
+    intros * abs.
+    unfold Exception.throw in *.
+    unfold interp_expr in *.
+    setoid_rewrite interp_Mem_vis_eqit in abs.
+    unfold pure_state in *; cbn in *.
+    rewrite interp_fail_bind in abs.
+    rewrite interp_fail_vis in abs.
+    cbn in *.
+    rewrite Eq.bind_bind, !bind_ret_l in abs.
+    rewrite translate_ret in abs.
+    eapply eutt_Ret in abs.
+    apply abs; auto.
+  Qed.
+
+  Lemma failure_expr_throw' : forall E s (k : uval -> _) m,
+    ~ no_failure (interp_expr (E := E) (ITree.bind (throw s) k) m).
+  Proof.
+    intros * abs.
+    rewrite interp_expr_bind in abs.
+    eapply no_failure_bind_prefix, failure_expr_throw in abs; auto.
+  Qed.
+
+  Lemma no_failure_expr_bind_prefix : forall {E} (t : itree _ uval) (k : uval -> itree _ uval) m,
+    no_failure (interp_expr (E := E) (ITree.bind t k) m) ->
+    no_failure (interp_expr (E := E) t m).
+  Proof.
+    intros * NOFAIL.
+    rewrite interp_expr_bind in NOFAIL.
+    eapply no_failure_bind_prefix; eapply NOFAIL.
+  Qed.
+  
+  Lemma no_failure_expr_bind_continuation :
+    forall {E} (t : itree _ uval) (k : uval -> itree _ uval) m,
+      no_failure (interp_expr (E := E) (ITree.bind t k) m) ->
+      forall u m', Returns (E := E) (Some (m',u)) (interp_expr t m) -> 
+        no_failure (interp_expr (E := E) (k u) m').
+  Proof.
+    intros * NOFAIL * ISRET.
+    rewrite interp_expr_bind in NOFAIL.
+    eapply no_failure_bind_cont in NOFAIL; eauto.
+    apply NOFAIL.
+  Qed.
+
+End NoFailure.
