cogent/llvm/checker/coq/HelixLib/Codegen.v
@@ -1,0 +1,189 @@
+(* Taken from Helix's LLVMGen.Compiler.v *)
+
+Require Import Coq.Bool.Bool.
+Require Import Coq.Strings.String.
+Require Import Coq.Lists.List.
+
+Require Import Vellvm.Semantics.IntrinsicsDefinitions.
+Require Import Vellvm.Utils.Util.
+Require Import Vellvm.Utils.Error.
+Require Import Vellvm.Numeric.Floats.
+Require Import Vellvm.Semantics.TopLevel.
+Require Import Vellvm.Syntax.LLVMAst.
+
+Require Import Flocq.IEEE754.Binary.
+Require Import Flocq.IEEE754.Bits.
+
+Require Import Coq.Numbers.BinNums. (* for Z scope *)
+Require Import Coq.ZArith.BinInt.
+From Coq Require Import ZArith.
+
+Require Import ExtLib.Structures.Monads.
+Require Import HelixLib.ErrorWithState.
+
+Import ListNotations.
+Import MonadNotation.
+Open Scope monad_scope.
+
+Set Implicit Arguments.
+Set Strict Implicit.
+
+(* Both [String] and [List] define [(++)] notation. We use both.
+   To avoid implicit scoping, we re-define one for String *)
+Notation "x @@ y" := (String.append x y) (right associativity, at level 60) : string_scope.
+
+Notation Var := (texp typ).
+
+Section withErrorStateMonad.
+
+  Record IRState :=
+    mkIRState
+      {
+        block_count: nat ;
+        local_count: nat ;
+        void_count : nat ;
+        Γ: list Var
+      }.
+
+  Definition newState (arg:Var): IRState :=
+    {|
+      block_count := 0 ;
+      local_count := 0 ;
+      void_count  := 0 ;
+      Γ := [arg]
+    |}.
+
+  Definition cerr := errS IRState.
+
+  Definition setVars (s:IRState) (newvars:list Var): IRState :=
+    {|
+      block_count := block_count s ;
+      local_count := local_count s ;
+      void_count  := void_count s ;
+      Γ := newvars
+    |}.
+
+  (* Returns n-th varable from state or error if [n] index oob *)
+  Definition getStateVar (msg:string) (n:nat): cerr Var :=
+    st <- get ;;
+    option2errS msg (List.nth_error (Γ st) n).
+
+  Definition evalCErrS {St:Type} {A:Type} (c : errS St A) (initial : St) : cerr A :=
+    match c initial with
+    | inl msg => raise msg
+    | inr (s,v) => ret v
+    end.
+
+End withErrorStateMonad.
+
+Definition add_comments (b:block typ) (xs:list string): block typ :=
+  {|
+    blk_id    := blk_id b;
+    blk_phis  := blk_phis b;
+    blk_code  := blk_code b;
+    blk_term  := blk_term b;
+    blk_comments := match blk_comments b with
+                    | None => Some xs
+                    | Some ys => Some (ys++xs)
+                    end
+  |}.
+
+Definition add_comment (bs:list (block typ)) (xs:list string): list (block typ) :=
+  match bs with
+  | nil => nil
+  | b::bs => (add_comments b xs)::bs
+  end.
+
+Definition incBlockNamed (prefix:string): (cerr block_id) :=
+  st <- get  ;;
+  put
+    {|
+      block_count := S (block_count st);
+      local_count := local_count st ;
+      void_count := void_count st ;
+      Γ := Γ st
+    |} ;;
+  ret (Name (prefix ++ string_of_nat (block_count st))).
+
+Definition incBlock := incBlockNamed "b".
+
+Definition incLocalNamed (prefix:string): (cerr raw_id) :=
+  st <- get ;;
+  put
+    {|
+      block_count := block_count st ;
+      local_count := S (local_count st) ;
+      void_count  := void_count st ;
+      Γ := Γ st
+    |} ;;
+  ret (Name (prefix @@ string_of_nat (local_count st))).
+
+Definition incLocal := incLocalNamed "l".
+
+Definition incVoid: (cerr int) :=
+  st <- get ;;
+  put
+    {|
+      block_count := block_count st ;
+      local_count := local_count st ;
+      void_count  := S (void_count st) ;
+      Γ := Γ st
+    |} ;;
+  ret (Z.of_nat (void_count st)).
+
+Definition addVars (newvars: list Var): cerr unit :=
+  st <- get ;;
+  put
+    {|
+      block_count := block_count st ;
+      local_count := local_count st ;
+      void_count  := void_count st ;
+      Γ := newvars ++ Γ st
+    |}.
+
+Definition intrinsic_exp (d:declaration typ): exp typ :=
+  EXP_Ident (ID_Global (dc_name d)).
+
+(* TODO: move *)
+Fixpoint drop_err {A:Type} (n:nat) (lst:list A) : err (list A)
+  := match n, lst with
+     | O, xs => ret xs
+     | S n', (_::xs) => drop_err n' xs
+     | _, _ => raise "drop on empty list"
+     end.
+
+Definition dropVars (n: nat): cerr unit :=
+  st <- get ;;
+  Γ' <- err2errS (drop_err n (Γ st)) ;;
+  put {|
+      block_count := block_count st ;
+      local_count := local_count st ;
+      void_count  := void_count st ;
+      Γ := Γ'
+    |}.
+
+Definition swap_err {A:Type} (lst:list A) : err (list A)
+  := match lst with
+     | (x :: y :: xs) => ret (y :: x :: xs)
+     | _ => raise "drop on empty list"
+     end.
+
+(* Swap top most elements on list. Used in IMapLoopBody *)
+Definition swapVars : cerr unit :=
+  st <- get ;;
+  Γ' <- err2errS (swap_err (Γ st)) ;;
+  put {|
+      block_count := block_count st ;
+      local_count := local_count st ;
+      void_count  := void_count st ;
+      Γ := Γ'
+    |}.
+
+(* Result and list of blocks with entry point *)
+Definition segment:Type := Var * block_id * list (block typ).
+
+Definition body_non_empty_cast (body : list (block typ)) : cerr (block typ * list (block typ)) :=
+  match body with
+  | [] => raise "Attempting to generate a function containing no block"
+  | b::body => ret (b,body)
+  end.
