cogent/llvm/checker/coq/HelixLib/Correctness_Prelude.v
@@ -1,0 +1,397 @@
+(* Taken from Helix's LLVMGen.Correctness_Prelude.v *)
+
+(** * Correctness of the pass of compilation from FSHCOL to VIR
+
+We prove the correctness of the pass of compilation defined in the
+_Correctness.v_. The Admitted.is based on the Interaction Trees approach: the
+semantics of both languages are denoted in terms of trees further interpreted
+into a monad built atop of the itree one.
+
+The semantic equivalence is expressed in terms of a weak bisimulation over the
+resulting monad.
+
+**)
+
+(** * Prelude
+  This file essentially:
+  - setup export the module shared over the whole proof
+  - define the semantic domains over which we work
+  - define conveniences to work with relations involved in the proof
+  - define notations and automations easing the Admitted.effort
+*)
+
+Require Export Coq.Arith.Arith.
+Require Export Coq.Lists.List.
+Require Export Coq.Strings.String.
+Require Export Coq.Numbers.BinNums. (* for Z scope *)
+Require Export Coq.ZArith.BinInt.
+Require Export Psatz.
+
+Require Export HelixLib.Codegen.
+Require Export HelixLib.Vellvm_Utils.
+
+Require Export Vellvm.Utils.Tactics.
+Require Export Vellvm.Utils.AListFacts.
+Require Export Vellvm.Utils.Util.
+Require Export Vellvm.Utils.PostConditions.
+Require Export Vellvm.Utils.NoFailure.
+Require Export Vellvm.Utils.PropT.
+Require Export Vellvm.Utils.TFor.
+Require Export Vellvm.Syntax.LLVMAst.
+Require Export Vellvm.Syntax.AstLib.
+Require Export Vellvm.Syntax.Scope.
+Require Export Vellvm.Syntax.DynamicTypes.
+Require Export Vellvm.Syntax.TypToDtyp.
+Require Export Vellvm.Syntax.CFG.
+Require Export Vellvm.Syntax.Traversal.
+Require Export Vellvm.Syntax.SurfaceSyntax.
+Require Export Vellvm.Syntax.ScopeTheory.
+Require Export Vellvm.Semantics.Denotation.
+Require Export Vellvm.Semantics.LLVMEvents.
+Require Export Vellvm.Semantics.InterpretationStack.
+Require Export Vellvm.Semantics.TopLevel.
+Require Export Vellvm.Handlers.Handlers.
+Require Export Vellvm.Theory.InterpreterMCFG.
+Require Export Vellvm.Theory.InterpreterCFG.
+Require Export Vellvm.Theory.TopLevelRefinements.
+Require Export Vellvm.Theory.DenotationTheory.
+Require Export Vellvm.Theory.InstrLemmas.
+Require Export Vellvm.Theory.ExpLemmas.
+Require Export Vellvm.Theory.SymbolicInterpreter.
+
+Require Export ExtLib.Structures.Monads.
+Require Export ExtLib.Data.Map.FMapAList.
+Require Export ExtLib.Core.RelDec.
+
+Require Export ITree.Interp.TranslateFacts.
+Require Export ITree.Basics.CategoryFacts.
+Require Export ITree.Events.State.
+Require Export ITree.Events.StateFacts.
+Require Export ITree.Events.FailFacts.
+Require Export ITree.ITree.
+Require Export ITree.Eq.Eq.
+Require Export ITree.Basics.Basics.
+Require Export ITree.Events.Exception.
+Require Export ITree.Interp.InterpFacts.
+
+Require Export MathClasses.interfaces.canonical_names.
+Require Export MathClasses.misc.decision.
+
+Import AlistNotations.
+
+Open Scope string_scope.
+Open Scope char_scope.
+
+Set Implicit Arguments.
+Set Strict Implicit.
+
+Export D.
+
+Import ListNotations.
+Import MonadNotation.
+Local Open Scope monad_scope.
+
+Open Scope string_scope.
+Open Scope char_scope.
+Open Scope nat_scope.
+Import ListNotations.
+Import MonadNotation.
+Local Open Scope monad_scope.
+
+(** Semantic domains
+
+  - Facilities to work with the same interface of events on both sides through an outer trivial translation.
+  - Definition of the top level definition of FSHCOL's semantics by performing the initialization of the
+  state at a meta level.
+  TODO: Move this semantic component out of the Admitted.
+
+
+*)
+
+(* A couple of notations to avoid ambiguities while not having to worry about imports and qualified names *)
+Notation memoryV := memory_stack.
+
+Section EventTranslation.
+
+  (* We relate Helix trees and Vellvm trees at a point where their event signatures are still not empty.
+  To do so, we therefore relate them at the join of these signature, using [translate] to do so.
+  Unfortunately, since [vellvm] works over two different set of signatures depending whether
+  function calls are already resolved or not, we also need two joins here.
+
+  TODOYZ: Principle the approach and move it to [itrees]
+
+  NOTEYZ: An alternative would be to translate everything that remains into failure. That could also be
+          part of the library as a generic handler.
+  *)
+
+  (* Joined set of residual events for full programs *)
+  Definition E_mcfg : Type -> Type := (ExternalCallE +' PickE +' UBE +' DebugE +' FailureE).
+  (* Joined set of residual events for cfgs *)
+  Definition E_cfg : Type -> Type := (CallE +' PickE +' UBE +' DebugE +' FailureE). 
+
+  (* We therefore have the following resulting denotation functions. *)
+  (* On the Vellvm side, for [mcfg]: *)
+  Definition semantics_llvm_mcfg p : itree E_mcfg _ := model_to_L3 DTYPE_Void "main" main_args p.
+  (* Which get lifted to [toplevel_entity] as usual: *)
+  Definition semantics_llvm (prog: list (toplevel_entity typ (LLVMAst.block typ * list (LLVMAst.block typ)))) :=
+    semantics_llvm_mcfg (convert_types (mcfg_of_tle prog)).
+
+  Definition inject_signature {E} : void1 ~> E := fun _ (x:void1 _) => match x with end.
+  Hint Unfold inject_signature : core.
+
+End EventTranslation.
+
+Notation "'interp_cfg'"  := interp_cfg3. 
+Notation "'interp_mcfg'" := interp_mcfg3. 
+
+(** Smart constructors for states, predicates, relations  *)
+
+(* Facilities to refer to the return types of the various pieces of denotations we manipulate *)
+
+Section StateTypes.
+
+  Local Open Scope type_scope.
+
+  (* Return state of a denoted and interpreted [cfg].
+    Note the lack of local stack *)
+  Definition config_cfg
+    := memoryV * (local_env * (global_env)).
+
+  (* Constructor to avoid having to worry about the nesting *)
+  Definition mk_config_cfg m l g: config_cfg := (m,(l,g)).
+
+  (* Return state of a denoted and interpreted [mcfg] *)
+  Definition config_mcfg
+    := memoryV *
+      (local_env * @Stack.stack (local_env) * (global_env)).
+
+  (* Return state and value of a denoted and interpreted (open) [cfg].
+    Note the lack of local stack.
+    Note that we may return a [block_id] alternatively to a [uvalue]
+  *)
+  Definition config_cfg_T (T:Type): Type
+    := memoryV * (local_env * (global_env * T)).
+  Definition config_res_cfg
+    := config_cfg_T (block_id + uvalue).
+
+  (* Return state and value of a denoted and interpreted [mcfg]. *)
+  Definition config_mcfg_T (T:Type): Type
+    := memoryV * (local_env * @Stack.stack (local_env) * (global_env * T)).
+  Definition config_res_mcfg :=
+    config_mcfg_T uvalue.
+
+  (* -- Injections -- *)
+  (* The nested state transformers associate the products the other way,
+    we therefore define injections of memory states and values into return
+    types of computations.
+  *)
+  Definition mk_config_cfg_T (T:Type) (v:T): config_cfg -> (config_cfg_T T)
+    := fun '(m, (ρ, g)) => (m, (ρ, (g, v))).
+
+  Definition mk_config_mcfg_T (T:Type) (v:T): config_mcfg -> (config_mcfg_T T)
+    := fun '(m, (ρ, g)) => (m, (ρ, (g, v))).
+
+End StateTypes.
+
+(* TODOYZ : MOVE *)
+Definition conj_rel {A B : Type} (R S: A -> B -> Prop): A -> B -> Prop :=
+  fun a b => R a b /\ S a b.
+Infix "⩕" := conj_rel (at level 85, right associativity).
+
+(* Introduction pattern useful after [eutt_clo_bind] *)
+Ltac introR :=
+  intros [[?memH ?vH] |] (?memV & ?l & ?g & ?vV) ?PRE; [| now inv PRE].
+
+(** Admitted.automation *)
+
+Ltac unfolder_vellvm       := unfold Traversal.Endo_id.
+Ltac unfolder_vellvm_hyp h := unfold Traversal.Endo_id in h.
+Ltac unfolder_vellvm_all   := unfold Traversal.Endo_id in *.
+
+(* This tactic is quite dumb, and should be refined if needed, but does a good job at
+  reducing the success of a compilation unit to the success of all of its sub-operations.
+*)
+Ltac simp := repeat (inv_sum || inv_option || break_and || break_match_hyp).
+
+Section Add_Comment.
+
+  (* NOTEYZ:
+    Move this or a similar facility to Vellvm
+  *)
+  Lemma add_comment_preserves_num_blocks :
+    forall l comments blocks,
+      add_comment l comments ≡ blocks ->
+      List.length l ≡ List.length blocks.
+  Admitted.
+
+  Lemma add_comment_singleton :
+    forall l comments block,
+      add_comment l comments ≡ [block] ->
+      exists b, l ≡ [b].
+  Admitted.
+
+  Lemma add_comment_inputs :
+    forall (bs : ocfg typ) (comments : list string),
+      inputs (add_comment bs comments) ≡ inputs bs.
+  Admitted.
+
+  Lemma add_comment_outputs :
+    forall (bs : ocfg typ) (comments : list string),
+      outputs (add_comment bs comments) ≡ outputs bs.
+  Admitted.
+
+  Lemma add_comment_inputs_typ :
+    forall (bs : list (LLVMAst.block typ)) env (comments : list string),
+      inputs (convert_typ env (add_comment bs comments)) ≡ inputs (convert_typ env bs).
+  Admitted.
+
+  Lemma add_comment_outputs_typ :
+    forall (bs : list (LLVMAst.block typ)) env (comments : list string),
+      outputs (convert_typ env (add_comment bs comments)) ≡ outputs (convert_typ env bs).
+  Admitted.
+
+  Lemma wf_ocfg_bid_add_comment :
+    forall bks s,
+      wf_ocfg_bid (add_comment bks s) ->
+      wf_ocfg_bid bks.
+  Admitted.
+
+  Lemma denote_ocfg_eutt_bk :
+    forall b b' bk x,
+      blk_id b ≡ blk_id b' ->
+      (forall bid_from, denote_block b bid_from ≈ denote_block b' bid_from) ->
+      denote_ocfg (b::bk) x ≈ denote_ocfg (b'::bk) x.
+  Admitted.
+  Global Opaque denote_ocfg.
+
+  (* Lemma add_comment_eutt :
+    forall comments bks ids,
+      denote_ocfg (convert_typ [] (add_comment bks comments)) ids ≈ denote_ocfg (convert_typ [] bks) ids.
+  Proof.
+    intros comments bks ids.
+    destruct bks as [| b bks].
+    - cbn; reflexivity.
+    - simpl add_comment.
+      cbn.
+      apply denote_ocfg_eutt_bk; [reflexivity |].
+      intros.
+      destruct b.
+      unfold fmap, Fmap_block.
+      cbn.
+      rewrite 2 denote_block_unfold.
+      reflexivity.
+  Qed. *)
+
+End Add_Comment.
+
+Global Opaque interp_cfg3.
+
+(* Autorewrite and hint databases for more modular rewriting. *)
+(* "Normalizing" rewriting hint database. *)
+Hint Rewrite @translate_bind : itree.
+Hint Rewrite @interp_bind : itree.
+Hint Rewrite @bind_bind : itree.
+Hint Rewrite @bind_ret_l : itree.
+
+Hint Rewrite @translate_ret : itree.
+Hint Rewrite @interp_ret : itree.
+
+Hint Rewrite @translate_trigger : itree.
+Hint Rewrite @interp_trigger : itree.
+
+Hint Rewrite @interp_cfg3_bind : vellvm.
+Hint Rewrite interp_cfg3_ret : vellvm.
+Hint Rewrite interp_cfg3_GR : vellvm.
+Hint Rewrite interp_cfg3_LR : vellvm.
+
+Hint Rewrite @LU_to_exp_Global : vellvm.
+Hint Rewrite @LU_to_exp_Local : vellvm.
+Hint Rewrite @subevent_subevent : vellvm.
+Hint Rewrite @exp_to_instr_Global : vellvm.
+Hint Rewrite @exp_to_instr_Local : vellvm.
+Hint Rewrite @typ_to_dtyp_equation : vellvm.
+Hint Rewrite denote_code_nil : vellvm.
+Hint Rewrite denote_code_singleton : vellvm.
+
+Tactic Notation "rauto:R" :=
+  repeat (
+      match goal with
+      | |- eutt _ ?t _ => let x := fresh in remember t as x;
+                                          autorewrite with itree;
+                                          autorewrite with vellvm;
+                                          autorewrite with helix; subst x
+      end
+    ).
+
+Tactic Notation "rauto:L" :=
+  repeat (
+      match goal with
+      | |- eutt _ _ ?t => let x := fresh in remember t as x;
+                                          autorewrite with itree;
+                                          autorewrite with vellvm;
+                                          autorewrite with helix; subst x
+      end
+    ).
+
+Tactic Notation "rauto" := (repeat (autorewrite with itree; autorewrite with vellvm; autorewrite with helix)).
+Tactic Notation "rauto" "in" hyp(h) :=
+  (repeat (autorewrite with itree in h; autorewrite with vellvm in h; autorewrite with helix in h)).
+
+Module ProofMode.
+
+  (* Include ITreeNotations. *)
+  Notation "t1 ;; k" := (ITree.bind t1 k) (format "t1 ;; '//' k", at level 61, right associativity, only printing) : itree_scope.
+  Include VIR_Notations.
+  Include VIR_denotation_Notations.
+  Include eutt_Notations.
+  Notation "g '[' r ':' x ']'" := (alist_add r x g) (only printing, at level 10). 
+
+  (* Notation "⟦ b , p , c , t ⟧" := (fmap _ (mk_block b p c t _)) (only printing).  *)
+  (* Notation "'denote_blocks' '...' id " := (denote_bks _ id) (at level 10,only printing).  *)
+  (* Notation "'IRS' ctx" := (mkIRState _ _ _ ctx) (only printing, at level 10).  *)
+  (* Notation "x" := (with_cfg x) (only printing, at level 10).  *)
+  (* Notation "x" := (with_mcfg x) (only printing, at level 10).  *)
+  (* (* Notation "'CODE' c" := (denote_code c) (only printing, at level 10, format "'CODE' '//' c"). *) *)
+  (* Notation "c" := (denote_code c) (only printing, at level 10). *)
+  (* (* Notation "'INSTR' i" := (denote_instr i) (only printing, at level 10, format "'INSTR' '//' i"). *) *)
+  (* Notation "i" := (denote_instr i) (only printing, at level 10). *)
+  (* Notation "x" := (translate exp_E_to_instr_E (denote_exp _ x)) (only printing, at level 10).  *)
+  
+End ProofMode.
+
+Ltac vred := vred_r.
+
+Require Import LibHyps.LibHyps.
+
+Ltac clean_goal :=
+  try match goal with
+      | h1 : incVoid _ ≡ _,
+            h2 : incVoid _ ≡ _,
+                  h3 : incVoid _ ≡ _
+        |- _ => move h1 at top; move h2 at top; move h3 at top
+      | h1 : incVoid _ ≡ _, h2 : incVoid _ ≡ _ |- _ => move h1 at top; move h2 at top
+      | h : incVoid _ ≡ _ |- _ => move h at top
+      end;
+
+  try match goal with
+      | h1 : incLocal _ ≡ _,
+            h2 : incLocal _ ≡ _,
+                  h3 : incLocal _ ≡ _
+        |- _ => move h1 at top; move h2 at top; move h3 at top
+      | h1 : incLocal _ ≡ _, h2 : incLocal _ ≡ _ |- _ => move h1 at top; move h2 at top
+      | h : incLocal _ ≡ _ |- _ => move h at top
+      end;
+
+  try match goal with
+      | h1 : incBlockNamed _ _ ≡ _,
+            h2 : incBlockNamed _ _ ≡ _,
+                  h3 : incBlockNamed _ _ ≡ _
+        |- _ => move h1 at top; move h2 at top; move h3 at top
+      | h1 : incBlockNamed _ _ ≡ _, h2 : incBlockNamed _ _ ≡ _ |- _ => move h1 at top; move h2 at top
+      | h : incBlockNamed _ _ ≡ _ |- _ => move h at top
+      end;
+
+  onAllHyps move_up_types.
+
+Arguments alist_add : simpl never.
+Arguments String.append : simpl never.
