cogent/llvm/checker/coq/HelixLib/IdLemmas.v
@@ -1,0 +1,99 @@
+(* Taken from Helix's LLVMGen.IdLemmas.v *)
+
+(** * Valid identifiers
+
+  When generating variable and block id names, we allow any purely alphabetical prefix
+  to be appended with the current freshness generator.
+  
+  The predicate [is_correct_prefix] is used to check prefixes. It computes and can therefore always simply be discharged by [reflexivity].
+  In particular [solve_prefix] takes care of it.
+
+  The main result of this file is [valid_prefix_neq_differ] ensuring that the variables we generate are distinct without having to worry about the prefixes.
+
+*)
+
+Require Import HelixLib.Correctness_Prelude.
+
+Set Implicit Arguments.
+Set Strict Implicit.
+
+Import  Ascii. 
+Definition is_connector (c : ascii) : bool :=
+  match c with
+  | "095" => true
+  | _ => false
+  end.
+
+Definition is_alpha (c : ascii) : bool :=
+  if CeresString.is_upper c then true else if
+      CeresString.is_lower c then true else
+      if is_connector c then true else false.
+
+Definition is_correct_prefix (s : string) : bool :=
+  CeresString.string_forall is_alpha s.
+
+Lemma string_forall_forallb (f : ascii → bool) (s : string) :
+    CeresString.string_forall f s
+    <->
+    forallb f (list_ascii_of_string s).
+Admitted.
+
+Lemma list_ascii_of_string_append :
+  forall s1 s2,
+    list_ascii_of_string (s1 @@ s2) ≡
+    List.app (list_ascii_of_string s1) (list_ascii_of_string s2).
+Admitted.
+
+Lemma string_forall_append (f : ascii → bool) (s1 s2 : string) :
+  CeresString.string_forall f s1 ->
+  CeresString.string_forall f s2 ->
+  CeresString.string_forall f (s1 @@ s2).
+Admitted.
+
+Lemma string_of_nat_not_alpha : forall n,
+  CeresString.string_forall (fun c => negb (is_alpha c)) (string_of_nat n).
+Admitted.
+
+Lemma is_correct_prefix_String : forall c s,
+    is_correct_prefix (String c s) ->
+    is_correct_prefix s /\ is_alpha c.
+Admitted.
+
+Import Ascii String.
+
+Lemma valid_prefix_string_of_nat_aux :
+  forall n k s,
+    is_correct_prefix s ->
+    string_of_nat n ≡ s @@ string_of_nat k ->
+    n ≡ k /\ s ≡ EmptyString.
+Admitted.
+
+Lemma valid_prefix_string_of_nat_forward :
+  forall s1 s2 n k,
+    is_correct_prefix s1 ->
+    is_correct_prefix s2 ->
+    s1 @@ string_of_nat n ≡ s2 @@ string_of_nat k ->
+    n ≡ k /\ s1 ≡ s2.
+Admitted.
+      
+Lemma valid_prefix_neq_differ :
+  forall s1 s2 n k,
+    is_correct_prefix s1 ->
+    is_correct_prefix s2 ->
+    n ≢ k ->
+    s1 @@ string_of_nat n ≢ s2 @@ string_of_nat k.
+Admitted.
+
+Lemma is_correct_prefix_append: forall s1 s2,
+    is_correct_prefix s1 ->
+    is_correct_prefix s2 ->
+    is_correct_prefix (s1 @@ s2).
+Admitted.
+
+Hint Resolve is_correct_prefix_append : PREFIX.
+
+Ltac solve_prefix :=
+  try solve
+      [ eauto with PREFIX
+      | now (unfold append; cbn; reflexivity)
+      ].
