cogent/llvm/checker/coq/HelixLib/StateCounters.v
@@ -1,0 +1,189 @@
+(* Taken from Helix's LLVMGen.StateCounters.v *)
+
+(** * Compilation units and IRState
+
+  This file contains a bunch of lemmas describing how various compilation subroutines
+  impact the freshness part of the [IRState].
+  The file [Context.v] is the pendant for the context part of the [IRState].
+*)
+
+Require Import HelixLib.Correctness_Prelude.
+
+Import ListNotations.
+
+Set Implicit Arguments.
+Set Strict Implicit.
+
+Section BlockCount.
+
+  Lemma incVoid_block_count :
+    forall s1 s2 bid,
+      incVoid s1 ≡ inr (s2, bid) ->
+      block_count s1 ≡ block_count s2.
+  Admitted.
+
+  Lemma incLocal_block_count :
+    forall s1 s2 bid,
+      incLocal s1 ≡ inr (s2, bid) ->
+      block_count s1 ≡ block_count s2.
+  Admitted.
+
+  Lemma incLocalNamed_block_count :
+    forall s s1 s2 bid,
+      incLocalNamed s s1 ≡ inr (s2, bid) ->
+      block_count s1 ≡ block_count s2.
+  Admitted.
+
+  Lemma incBlockNamed_block_count:
+    forall s s' msg id,
+      incBlockNamed msg s ≡ inr (s', id) ->
+      block_count s' ≡ S (block_count s).
+  Admitted.
+
+  Lemma dropVars_block_count :
+    ∀ (s1 s2 : IRState) bid x,
+      dropVars x s1 ≡ inr (s2, bid) →
+      block_count s1 ≡ block_count s2.
+  Admitted.
+
+  Ltac __local_ltac' := (repeat
+      (match goal with
+      | H: inl _ ≡ inr _ |- _ =>
+        inversion H
+      | H: ErrorWithState.option2errS _ (nth_error (Γ ?s1) ?n) ?s1 ≡ inr (?s2, _) |- _ =>
+        destruct (nth_error (Γ s1) n) eqn:?; inversion H; subst
+      | H : incLocal ?s1 ≡ inr (?s2, _) |- _ =>
+        apply incLocal_block_count in H
+      | H : incVoid ?s1 ≡ inr (?s2, _) |- _ =>
+        apply incVoid_block_count in H
+      | H : incBlockNamed _ _ ≡ inr _ |- _ =>
+        apply incBlockNamed_block_count in H
+      | H : incBlock _ ≡ inr _ |- _ =>
+        apply incBlockNamed_block_count in H
+      end; cbn in *)).
+
+  Opaque incLocal.
+  Opaque incVoid.
+  Opaque incBlockNamed.
+
+End BlockCount.
+      
+Section LocalCount.
+
+  Lemma incBlockNamed_local_count:
+    forall s s' msg id,
+      incBlockNamed msg s ≡ inr (s', id) ->
+      local_count s' ≡ local_count s.
+  Admitted.
+
+  Lemma incVoid_local_count:
+    forall s s' id,
+      incVoid s ≡ inr (s', id) ->
+      local_count s' ≡ local_count s.
+  Admitted.
+
+  Lemma incLocal_local_count: forall s s' x,
+      incLocal s ≡ inr (s',x) ->
+      local_count s' ≡ S (local_count s).
+  Admitted.
+
+  Lemma dropVars_local_count:
+    forall s s' k,
+      dropVars k s ≡ inr (s', tt) ->
+      local_count s' ≡ local_count s.
+  Admitted.
+
+  Lemma incLocalNamed_local_count: forall s s' msg x,
+      incLocalNamed msg s ≡ inr (s',x) ->
+      local_count s' ≡ S (local_count s).
+  Admitted.
+
+  Opaque incLocal.
+  Opaque incVoid.
+  Opaque incBlockNamed.
+  Arguments append: simpl never.
+
+  Ltac __local_ltac :=
+    repeat
+      (match goal with
+      | H: inl _ ≡ inr _ |- _ =>
+        inversion H
+      | H: ErrorWithState.option2errS _ (nth_error (Γ ?s1) ?n) ?s1 ≡ inr (?s2, _) |- _ =>
+        destruct (nth_error (Γ s1) n) eqn:?; inversion H; subst
+      | H : incLocal ?s1 ≡ inr (?s2, _) |- _ =>
+        apply incLocal_local_count in H
+      | H : incVoid ?s1 ≡ inr (?s2, _) |- _ =>
+        apply incVoid_local_count in H
+        | H : incBlockNamed _ _ ≡ inr _ |- _ =>
+        apply incBlockNamed_local_count in H
+      | H : incBlock _ ≡ inr _ |- _ =>
+        apply incBlockNamed_local_count in H
+      end; cbn in *).
+
+End LocalCount.
+
+  (* (* We define the obvious total order on IRStates *) *)
+  (* Definition IRState_lt (s1 s2 : IRState) : Prop := *)
+  (*   (local_count s1 < local_count s2)%nat. *)
+  (* Infix "<<" := IRState_lt (at level 10). *)
+
+  (* Definition IRState_le (s1 s2 : IRState) : Prop := *)
+  (*   (local_count s1 <= local_count s2)%nat. *)
+  (* Infix "<<=" := IRState_le (at level 10). *)
+
+  (* Lemma incLocal_lt : forall s1 s2 x, *)
+  (*     incLocal s1 ≡ inr (s2,x) -> *)
+  (*     s1 << s2. *)
+  (* Proof. *)
+  (*   intros s1 s2 x INC. *)
+  (*   apply incLocal_local_count in INC. *)
+  (*   unfold IRState_lt. *)
+  (*   lia. *)
+  (* Qed. *)
+
+  (* Create HintDb irs_lt. *)
+  (* Hint Resolve incLocal_lt : irs_lt. *)
+
+
+  (* Tactics *)
+
+Ltac get_local_count_hyps :=
+  repeat
+    match goal with
+    | H: incBlockNamed ?n ?s1 ≡ inr (?s2, _) |- _ =>
+      apply incBlockNamed_local_count in H; cbn in H
+    | H: incLocalNamed ?n ?s1 ≡ inr (?s2, _) |- _ =>
+      apply incLocalNamed_local_count in H; cbn in H
+    | H: incVoid ?s1 ≡ inr (?s2, _) |- _ =>
+      apply incVoid_local_count in H; cbn in H
+    | H: incLocal ?s1 ≡ inr (?s2, _) |- _ =>
+      apply incLocal_local_count in H; cbn in H
+    | H: dropVars _ ?s1 ≡ inr (?s2, _) |- _ =>
+      apply dropVars_local_count in H; cbn in H
+    end.
+
+Ltac get_block_count_hyps :=
+  repeat
+    match goal with
+    | H: incBlockNamed ?n ?s1 ≡ inr (?s2, _) |- _ =>
+      apply incBlockNamed_block_count in H; cbn in H
+    | H: incLocalNamed ?n ?s1 ≡ inr (?s2, _) |- _ =>
+      apply incLocalNamed_block_count in H; cbn in H
+    | H: incVoid ?s1 ≡ inr (?s2, _) |- _ =>
+      apply incVoid_block_count in H; cbn in H
+    | H: incLocal ?s1 ≡ inr (?s2, _) |- _ =>
+      apply incLocal_block_count in H; cbn in H
+    | H: dropVars _ ?s1 ≡ inr (?s2, _) |- _ =>
+      apply dropVars_block_count in H; cbn in H
+    end.
+
+Ltac solve_local_count := try solve [ cbn; get_local_count_hyps; lia
+                                    | reflexivity
+                                    ].
+
+Ltac solve_block_count := try solve [ cbn; get_block_count_hyps; lia
+                                    | reflexivity
+                                    ].
+
+Notation "s1 << s2" := (local_count s1 < local_count s2) (at level 50).
+Notation "s1 <<= s2" := (local_count s1 <= local_count s2) (at level 50).
