cogent/llvm/checker/coq/HelixLib/Vellvm_Utils.v
@@ -1,0 +1,174 @@
+(* Taken from Helix's LLVMGen.Vellvm_Utils.v *)
+
+From ITree Require Import
+     ITree
+     ITreeFacts
+     Events.State
+     Events.StateFacts
+     InterpFacts
+     Eq.Eq.
+
+From Vellvm Require Import
+     Utils.Tactics
+     Utils.Util
+     Syntax.LLVMAst
+     Syntax.Traversal
+     Syntax.AstLib
+     Syntax.DynamicTypes
+     Syntax.CFG
+     Syntax.TypToDtyp
+     Semantics.LLVMEvents
+     Semantics.DynamicValues
+     Semantics.TopLevel
+     Semantics.InterpretationStack
+     Handlers.Handlers
+     Theory.Refinement
+     Theory.DenotationTheory
+     Theory.InterpreterCFG.
+
+From ExtLib Require Import
+     Structures.Functor.
+
+From Coq Require Import
+     Strings.String
+     Logic
+     Morphisms
+     Relations
+     List.
+
+Require Import Ceres.Ceres.
+Import BinInt.
+Import ListNotations.
+Import ITree.Basics.Basics.Monads.
+
+From Vellvm Require Import Util.
+Require Import ITree.Events.State.
+
+Require Import ITree.Eq.Eq.
+
+From Vellvm Require Import Utils.AListFacts.
+
+Import Traversal.
+
+(* YZ: Should they be Opaque or simpl never? *)
+Global Opaque denote_ocfg.
+Global Opaque assoc.
+Global Opaque denote_instr.
+Global Opaque denote_terminator.
+Global Opaque denote_phi.
+Global Opaque denote_code.
+
+Ltac typ_to_dtyp_simplify :=
+  repeat
+    (try rewrite typ_to_dtyp_I in *;
+     try rewrite typ_to_dtyp_D in *;
+     try rewrite typ_to_dtyp_D_array in *;
+     try rewrite typ_to_dtyp_P in *).
+
+From Paco Require Import paco.
+Lemma eutt_mon {E R1 R2} (RR RR' : R1 -> R2 -> Prop)
+      (LERR: RR <2= RR') :
+  @eutt E R1 R2 RR <2= eutt RR'.
+Proof.
+  eapply eqit_mon; eauto.
+Qed.
+
+From Vellvm Require Import Syntax.Scope.
+
+(* Enforcing these definitions to be unfolded systematically by [cbn] *)
+Arguments endo /.
+Arguments Endo_id /.
+Arguments Endo_ident /.
+
+Arguments find_block : simpl never.
+
+From Vellvm Require Import Theory.SymbolicInterpreter.
+
+Module eutt_Notations.
+  Notation "t '======================' '======================' u '======================' '{' R '}'"
+    := (eutt R t u)
+         (only printing, at level 200,
+          format "'//' '//' t '//' '======================' '======================' '//' u '//' '======================' '//' '{' R '}'"
+         ).
+End eutt_Notations.
+
+Import D. 
+Module VIR_denotation_Notations.
+  (* Notation "'ℐ' '(' t ')' g l m" := (interp_cfg_to_L3 _ t g l m) (only printing, at level 10). *)
+  Notation "'global.' g 'local.' l 'memory.' m 'ℐ' t" :=
+    (interp_cfg3 t g l m)
+      (only printing, at level 10,
+       format "'global.'  g '//' 'local.'  l '//' 'memory.'  m '//' 'ℐ'  t").
+  
+  Notation "⟦ c ⟧" := (denote_code c) (only printing, at level 10).
+  Notation "⟦ i ⟧" := (denote_instr i) (only printing, at level 10).
+  Notation "⟦ t ⟧" := (denote_terminator t) (only printing, at level 10).
+  Notation "⟦ e ⟧" := (denote_exp None e) (only printing, at level 10).
+  Notation "⟦ τ e ⟧" := (denote_exp (Some τ) e) (only printing, at level 10).
+  Notation "x" := (translate exp_to_instr x) (only printing, at level 10).
+
+  Notation "'λ' a b c d ',' k" := (fun '(a,(b,(c,d))) => k) (only printing, at level 0, format "'λ'  a  b  c  d ',' '[' '//' k ']'").
+
+End VIR_denotation_Notations.
+
+Import ITreeNotations.
+
+From Vellvm Require Import InstrLemmas ExpLemmas.
+
+Ltac vred_r :=
+  let R := fresh
+  in eutt_hide_rel_named R;
+     let X := fresh
+     in eutt_hide_left_named X; vred_C3;
+        subst X; subst R.
+
+Ltac vred_l :=
+  let R := fresh
+  in eutt_hide_rel_named R;
+     let X := fresh
+     in eutt_hide_right_named X; vred_C3;
+        subst X; subst R.
+
+Ltac vstep := vstep3.
+
+Ltac tred := autorewrite with itree.
+
+Arguments denote_exp : simpl never.
+(* TODO: fmap (mk_block _ _ _ _ _) does not reduce, although we would like.
+   However if I do the following to force the unfolding, then fmap always
+   unfolds even in many other cases where we don't want it to do so.
+   Solution?
+ *)
+(* Arguments fmap /. *)
+(* Arguments Fmap_block /. *)
+Arguments denote_phis : simpl never.
+Arguments denote_code : simpl never.
+Arguments denote_terminator : simpl never.
+Arguments denote_block : simpl never.
+
+From Vellvm Require Import
+     Utils.TFor
+     Utils.NoFailure
+     Utils.PropT
+.
+Require Export ITree.Events.FailFacts.
+
+From Coq Require Import Lia.
+
+(* TODO: tactics? *)
+Ltac solve_allocated :=
+  solve [ eauto
+        | eapply dtyp_fits_allocated; eauto
+        | eapply handle_gep_addr_allocated; cycle 1; [solve [eauto] | solve_allocated]
+        | eapply write_preserves_allocated; cycle 1; [solve [eauto] | solve_allocated]
+        ].
+
+Ltac solve_read :=
+  solve [ eauto
+        (* This is largely for cases where sizeof_dtyp t <> 0 -> read ... *)
+        | match goal with
+          | H: _ |- _ => apply H
+          end; cbn; lia
+        | (* read from an array *)
+        erewrite read_array; cycle 2; [solve [eauto] | | solve_allocated]; eauto
+        ].
