cogent/llvm/checker/coq/Invariants.v
@@ -1,0 +1,138 @@
+From Checker Require Import Cogent Compiler Denotation HelixLib.Correctness_Prelude HelixLib.LidBound.
+
+(* From ITree Require Import ITree ITreeFacts. *)
+
+From Vellvm Require Import DynamicValues.
+
+Set Implicit Arguments.
+Set Strict Implicit.
+
+Import ListNotations.
+Import AlistNotations.
+
+Notation memoryC := Denotation.memory.
+
+(* Based on Helix's LLVMGen.Correctness_Invariants.v *)
+Section HelixInvariantUtils.
+
+  Definition WF_IRState (γ : ctx) (s : IRState) : Prop :=
+    True.
+    (* evalContext_typechecks σ (Γ s). *)
+
+  (* Predicate stating that an (llvm) local variable is relevant to the memory invariant *)
+  Variant in_Gamma : ctx -> IRState -> raw_id -> Prop :=
+  | mk_in_Gamma : forall σ s id τ n v,
+      nth_error σ n ≡ Some v ->
+      nth_error (Γ s) n ≡ Some (τ, EXP_Ident (ID_Local id)) ->
+      WF_IRState σ s ->
+      in_Gamma σ s id.
+
+  (* Given an initial local env [l1] that reduced to [l2], and a range given by [s1;s2], ensures
+  that all modified variables came from this range *)
+  Definition local_scope_modif (s1 s2 : IRState) (l1 : local_env) : local_env -> Prop :=
+    fun l2 =>
+      forall id,
+        alist_find id l2 <> alist_find id l1 ->
+        lid_bound_between s1 s2 id.
+  
+  (* Given an initial local env [l1] that reduced to [l2], and a range given by [s1;s2], ensures
+  that this range has been left untouched *)
+  Definition local_scope_preserved (s1 s2 : IRState) (l1 : local_env) : local_env -> Prop :=
+    fun l2 => forall id,
+        lid_bound_between s1 s2 id ->
+        l2 @ id ≡ l1 @ id.
+
+  (* Given an initial local env [l1] that reduced to [l2], ensures that no variable relevant to the memory invariant has been modified *)
+  Definition Gamma_preserved γ s (l1 l2 : local_env) : Prop :=
+    forall id,
+      in_Gamma γ s id ->
+      l1 @ id ≡ l2 @ id.
+
+  (* If no change has been made, all changes are certainly in the interval *)
+  Lemma local_scope_modif_refl: forall s1 s2 l, local_scope_modif s1 s2 l l.
+  Admitted.
+
+  (* If all changes made are in the empty interval, then no change has been made *)
+  Lemma local_scope_modif_empty_scope:
+    forall (l1 l2 : local_env) id s,
+      local_scope_modif s s l1 l2 ->
+      l2 @ id ≡ l1 @ id.
+  Admitted.
+
+End HelixInvariantUtils.
+
+(* Based on some more stuff in Helix's Correctness_Prelude.v *)
+Section HelixRelations.
+
+  Local Open Scope type_scope.
+
+  Definition config_cogent := memoryC.
+  Definition config_cogent_O := option memoryC.
+
+  Definition config_cogent_T (T : Type) := memoryC * T.
+  Definition config_cogent_OT (T : Type) := option (memoryC * T).
+
+  Definition Rel_cfg : Type := config_cogent -> config_cfg -> Prop.
+  Definition Rel_cfg_T (A B : Type) : Type := config_cogent_T A -> config_cfg_T B -> Prop.
+  Definition Rel_cfg_OT (A B : Type) : Type := config_cogent_OT A -> config_cfg_T B -> Prop.
+
+  Definition lift_Rel_cfg {A B} (R : Rel_cfg) : Rel_cfg_T A B :=
+    fun '(c_mem, _) '(v_mem, (l, (g, _))) => R c_mem (v_mem, (l, g)).
+
+  Definition succ_rel_l {A B} (R : A -> B -> Prop) : option A -> B -> Prop :=
+    fun ma b => match ma with | Some a => R a b | _ => False end.
+  Definition succ_cfg {A B}: Rel_cfg_T A B -> Rel_cfg_OT A B := succ_rel_l.
+
+  Definition conj_rel {A B : Type} (R S: A -> B -> Prop): A -> B -> Prop :=
+    fun a b => R a b /\ S a b.
+
+End HelixRelations.
+
+Coercion succ_cfg : Rel_cfg_T >-> Rel_cfg_OT.
+
+Section ValueRelation.
+
+  Definition convert_uval (u : uval) : uvalue :=
+    match u with
+    | UPrim (LBool b) => UVALUE_I1 (Int1.repr (if b then 1 else 0))
+    | UPrim (LU8 w) => UVALUE_I8 (Int8.repr w)
+    | UPrim (LU32 w) => UVALUE_I32 (Int32.repr w)
+    | UPrim (LU64 w) => UVALUE_I64 (Int64.repr w)
+    | UUnit => UVALUE_I8 (Int8.repr 0)
+    end.
+
+  Definition correct_result (γ : ctx) (s1 s2 : IRState) (u : uval) (i : im) : config_cfg -> Prop :=
+    fun '(memV, (l, g)) =>
+      forall l',
+        local_scope_preserved s1 s2 l l' ->
+        Gamma_preserved γ s1 l l' ->
+        interp_cfg
+          (translate exp_to_instr (denote_exp (Some (typ_to_dtyp [] (fst i))) (convert_typ [] (snd i))))
+          g l' memV ≈
+          Ret (memV, (l',(g, convert_uval u))).
+
+  (* correct means: does i evaluate to something equivalent to u *)
+  Definition correct_result_T {T} (γ : ctx) (s1 s2 : IRState) (i : im) : Rel_cfg_T uval T :=
+    fun '(_, u) '(memV, (l, (g, _))) => correct_result γ s1 s2 u i (memV, (l, g)).
+
+End ValueRelation.
+
+Section Memory.
+
+  Definition memory_invariant (γ : ctx) (s : IRState) (cogent : config_cogent)
+                              (vellvm : state_cfg) : Prop :=
+    forall (n : nat) (i : im) (u : uval),
+      nth_error γ n ≡ Some u ->
+      nth_error (Γ s) n ≡ Some i ->
+      correct_result γ s s u i vellvm.
+
+End Memory.
+
+Section State.
+
+  Record state_invariant (γ : ctx) (s : IRState) (cogent : config_cogent) (vellvm : config_cfg) : Prop :=
+  { mem_is_inv : memory_invariant γ s cogent vellvm
+  ; IRState_is_WF : WF_IRState γ s
+  }.
+
+End State.
