cogent/llvm/checker/coq/Utils/Tactics.v
@@ -1,217 +1,26 @@
-(* From Helix. To clean up *)
+From Checker Require Import DenotationTheory HelixLib.Correctness_Prelude.
 
-From Coq Require Export Arith List String BinNums BinInt.
-Require Export Psatz.
+(* From Helix *)
 
-From Vellvm Require Export Syntax.Traversal Utils.Error Utils.Tactics.
+Ltac unfolder_cogent       := unfold ErrorWithState.option2errS, ErrorWithState.err2errS.
+Ltac unfolder_cogent_hyp h := unfold ErrorWithState.option2errS, ErrorWithState.err2errS in h.
+Ltac unfolder_cogent_all   := unfold ErrorWithState.option2errS, ErrorWithState.err2errS in *.
 
-From Checker Require Import Utils.Codegen Utils.ErrorWithState.
-
-
-(* Introduction pattern useful after [eutt_clo_bind] *)
-(* Ltac introR :=
-  intros [[?memH ?vH] |] (?memV & ?l & ?g & ?vV) ?PRE; [| now inv PRE]. *)
-
-(** Proof automation *)
-
-Ltac unfolder_vellvm       := unfold Traversal.Endo_id.
-Ltac unfolder_vellvm_hyp h := unfold Traversal.Endo_id in h.
-Ltac unfolder_vellvm_all   := unfold Traversal.Endo_id in *.
-
-Ltac unfolder_helix       := unfold option2errS, err2errS, trywith.
-Ltac unfolder_helix_hyp h := unfold option2errS, err2errS, trywith in h.
-Ltac unfolder_helix_all   := unfold option2errS, err2errS, trywith in *.
-
-(**
-     Better solution (?): use
-     `Argument myconstant /.`
-     to force `cbn` to unfold `myconstant`
- *)
-Tactic Notation "unfolder" := unfolder_helix; unfolder_vellvm.
-Tactic Notation "unfolder" "in" hyp(h) := unfolder_helix_hyp h; unfolder_vellvm_hyp h.
-Tactic Notation "unfolder" "in" "*" := unfolder_helix_all; unfolder_vellvm_all.
+Tactic Notation "unfolder" := unfolder_cogent; unfolder_vellvm.
+Tactic Notation "unfolder" "in" hyp(h) := unfolder_cogent_hyp h; unfolder_vellvm_hyp h.
+Tactic Notation "unfolder" "in" "*" := unfolder_cogent_all; unfolder_vellvm_all.
 
 Tactic Notation "cbn*" := (repeat (cbn; unfolder)).
 Tactic Notation "cbn*" "in" hyp(h) := (repeat (cbn in h; unfolder in h)).
 Tactic Notation "cbn*" "in" "*" := (repeat (cbn in *; unfolder in *)).
 
-(* This tactic is quite dumb, and should be refined if needed, but does a good job at
-   reducing the success of a compilation unit to the success of all of its sub-operations.
- *)
-Ltac simp := repeat (inv_sum || inv_option || break_and || break_match_hyp).
-
-
-
-
-From ITree Require Import
-     ITree
-     ITreeFacts
-     Events.State
-     Events.StateFacts
-     InterpFacts
-     Eq.Eq.
-
-From Vellvm Require Import
-     Utils.Tactics
-     Utils.Util
-     Syntax.LLVMAst
-     Syntax.Traversal
-     Syntax.AstLib
-     Syntax.DynamicTypes
-     Syntax.CFG
-     Syntax.TypToDtyp
-     Semantics.LLVMEvents
-     Semantics.DynamicValues
-     Semantics.TopLevel
-     Semantics.InterpretationStack
-     Handlers.Handlers
-     Theory.Refinement
-     Theory.DenotationTheory
-     Theory.InterpreterCFG.
-
-From ExtLib Require Import
-     Structures.Functor.
-
-From Coq Require Import
-     Strings.String
-     Logic
-     Morphisms
-     Relations
-     List.
-
-Require Import Ceres.Ceres.
-Import BinInt.
-Import ListNotations.
-Import ITree.Basics.Basics.Monads.
-
-From Vellvm Require Import Util.
-Require Import ITree.Events.State.
-
-Require Import ITree.Eq.Eq.
-
-From Vellvm Require Import Utils.AListFacts.
-
-Import Traversal.
-
-(* YZ: Should they be Opaque or simpl never? *)
-Global Opaque denote_ocfg.
-Global Opaque assoc.
-Global Opaque denote_instr.
-Global Opaque denote_terminator.
-Global Opaque denote_phi.
-Global Opaque denote_code.
-
-Ltac typ_to_dtyp_simplify :=
-  repeat
-    (try rewrite typ_to_dtyp_I in *;
-     try rewrite typ_to_dtyp_D in *;
-     try rewrite typ_to_dtyp_D_array in *;
-     try rewrite typ_to_dtyp_P in *).
-
-From Paco Require Import paco.
-Lemma eutt_mon {E R1 R2} (RR RR' : R1 -> R2 -> Prop)
-      (LERR: RR <2= RR') :
-  @eutt E R1 R2 RR <2= eutt RR'.
-Proof.
-  eapply eqit_mon; eauto.
-Qed.
-
-From Vellvm Require Import Syntax.Scope.
-
-(* Enforcing these definitions to be unfolded systematically by [cbn] *)
-Arguments endo /.
-Arguments Endo_id /.
-Arguments Endo_ident /.
-
-Arguments find_block : simpl never.
-
-From Vellvm Require Import Theory.SymbolicInterpreter.
-
-Module eutt_Notations.
-  Notation "t '======================' '======================' u '======================' '{' R '}'"
-    := (eutt R t u)
-         (only printing, at level 200,
-          format "'//' '//' t '//' '======================' '======================' '//' u '//' '======================' '//' '{' R '}'"
-         ).
-End eutt_Notations.
-
-Import D. 
-Module VIR_denotation_Notations.
-  (* Notation "'ℐ' '(' t ')' g l m" := (interp_cfg_to_L3 _ t g l m) (only printing, at level 10). *)
-  Notation "'global.' g 'local.' l 'memory.' m 'ℐ' t" :=
-    (interp_cfg3 t g l m)
-      (only printing, at level 10,
-       format "'global.'  g '//' 'local.'  l '//' 'memory.'  m '//' 'ℐ'  t").
-  
-  Notation "⟦ c ⟧" := (denote_code c) (only printing, at level 10).
-  Notation "⟦ i ⟧" := (denote_instr i) (only printing, at level 10).
-  Notation "⟦ t ⟧" := (denote_terminator t) (only printing, at level 10).
-  Notation "⟦ e ⟧" := (denote_exp None e) (only printing, at level 10).
-  Notation "⟦ τ e ⟧" := (denote_exp (Some τ) e) (only printing, at level 10).
-  Notation "x" := (translate exp_to_instr x) (only printing, at level 10).
-
-  Notation "'λ' a b c d ',' k" := (fun '(a,(b,(c,d))) => k) (only printing, at level 0, format "'λ'  a  b  c  d ',' '[' '//' k ']'").
-
-End VIR_denotation_Notations.
-
-Import ITreeNotations.
-
-From Vellvm Require Import InstrLemmas ExpLemmas.
-
-Ltac vred_r :=
+Ltac cred :=
   let R := fresh
   in eutt_hide_rel_named R;
-     let X := fresh
-     in eutt_hide_left_named X; vred_C3;
-        subst X; subst R.
+    let X := fresh
+    in eutt_hide_right_named X;
+      repeat (rewrite ?interp_expr_bind, ?interp_expr_Ret, ?bind_ret_l);
+      subst R; subst X.
 
-Ltac vred_l :=
-  let R := fresh
-  in eutt_hide_rel_named R;
-     let X := fresh
-     in eutt_hide_right_named X; vred_C3;
-        subst X; subst R.
-
-Ltac vstep := vstep3.
-
-Ltac tred := autorewrite with itree.
-
-Arguments denote_exp : simpl never.
-(* TODO: fmap (mk_block _ _ _ _ _) does not reduce, although we would like.
-   However if I do the following to force the unfolding, then fmap always
-   unfolds even in many other cases where we don't want it to do so.
-   Solution?
- *)
-(* Arguments fmap /. *)
-(* Arguments Fmap_block /. *)
-Arguments denote_phis : simpl never.
-Arguments denote_code : simpl never.
-Arguments denote_terminator : simpl never.
-Arguments denote_block : simpl never.
-
-From Vellvm Require Import
-     Utils.TFor
-     Utils.NoFailure
-     Utils.PropT
-.
-Require Export ITree.Events.FailFacts.
-
-From Coq Require Import Lia.
-
-From Checker Require Import Denote.
-
-Ltac hred :=
-    let R := fresh
-    in eutt_hide_rel_named R;
-        let X := fresh
-        in eutt_hide_right_named X;
-            repeat (rewrite ?interp_expr_bind, ?interp_expr_Ret, ?bind_ret_l);
-            subst R; subst X.
-    
-    (* Ltac hstep := first [rewrite interp_helix_MemSet | rewrite interp_helix_MemLU; cycle 1 | idtac]. *)
-    
 Ltac vred := vred_r.
-Ltac hvred := hred; vred_r.
-
-Ltac introR :=
-  intros [[?memC ?vC] |] (?memV & ?l & ?g & ?vV) ?PRE; [| now inv PRE].
+Ltac cvred := cred; vred_r.
